\documentclass{article}
\usepackage{hwopt}
\usepackage{amsmath}	% Package for AMS
\usepackage{amsthm}     % Package for AMS-therom
\usepackage{amssymb}	% Package for AMS-symbol
\usepackage{bm}

\newcommand{\xB}{\bm{x}}
\newcommand{\yB}{\bm{y}}
\newcommand{\gB}{\bm{g}}
\newcommand{\RBB}{\mathbb{R}}
\newcommand{\FM}{\mathcal{F}}
\newcommand{\SM}{\mathcal{S}}
\newcommand{\LM}{\mathcal{L}}
\newcommand{\domf}{\textrm{dom}\;f}
\newcommand{\functiontype}[3]{\FM_{#1}^{#2,#3}(\RBB^n)}
\newcommand{\normgen}[1]{\left\| #1 \right\|}
\newcommand{\strongconvextype}[2]{\SM_{#1}^{#2}(\RBB^n)}
\newcommand{\argmin}{\mathop{\rm argmin}}

%%%%%%%%%%%%%%%%%
%     Title     %
%%%%%%%%%%%%%%%%%
\title{Coursework (5) for \emph{Introductory Lectures on Optimization}}
\author{Zhou Nan \\ 3220102535}
\date{\today}

\begin{document}
\maketitle

\begin{excercise}\label{e0}
Prove the following theorem: \\
for any $\xB_0 \in \domf$, all vectors $\gB \in \partial f(\xB_0)$ are supporting to the level set $\LM_f (f(\xB_0))$:
\begin{equation}
	\innerproduct{\gB}{\xB_0 - \xB} \geq 0, \;\;\; \forall \xB \in \LM_f(f(\xB_0)) \equiv \{ \xB \in \domf: f(\xB) \leq f(\xB_0) \}.\nonumber
\end{equation}
\end{excercise}
\begin{PROOF}{e0}
	According to the definition of subdifferential, we have

	\[
	f(\bm{x}) \geq f(\bm{x}_0) + \langle \bm{g}, \bm{x} - \bm{x}_0 \rangle
	\]
	
	Then, for any \(\bm{x} \in \mathcal{L}_f(f(\bm{x}_0))\), we have
	\[
		f(\bm{x}) \leq f(\bm{x}_0)
	\]
	Therefore,
	\[
	\langle \bm{g}, \bm{x} - \bm{x}_0 \rangle \leq f(\bm{x}) - f(\bm{x}_0) \leq 0.
	\]
	
	\[
	\langle \bm{g}, \bm{x}_0 - \bm{x} \rangle \geq 0.
	\]
	
	Therefore, for any $\xB_0 \in \domf$, all vectors $\gB \in \partial f(\xB_0)$ are supporting to the level set $\LM_f (f(\xB_0))$.
\end{PROOF}

\begin{excercise}\label{e1}
Prove the following theorem: \\
let $Q \subseteq \domf$ be a closed convex set,  $\xB_0 \in Q$ and 
 \begin{equation}
 	\xB^* = \argmin \{ f(\xB) | \xB \in Q \}.\nonumber
 \end{equation}
 Then for any $g \in \partial f(\xB_0)$ we have $\innerproduct{\gB}{\xB_0 - \xB^*} \geq 0$.
\end{excercise}
\begin{PROOF}{e1}
	According to the definition of subdifferential, we have

	\[
	f(\bm{x}) \geq f(\bm{x}_0) + \langle \bm{g}, \bm{x} - \bm{x}_0 \rangle
	\]
	Then, for any $\bm{x} = \xB^* \in Q$, we have
	\[
	f(\bm{x}^*) \leq f(\bm{x_0})
	\]
	Therefore,
	\[
	\langle \bm{g}, \bm{x}^* - \bm{x}_0 \rangle \leq f(\bm{x}^*) - f(\bm{x}_0) \leq 0
	\]
	\[
	\langle \bm{g}, \bm{x}_0 - \bm{x}^* \rangle \geq 0
	\]
\end{PROOF}

\begin{excercise}\label{e2}
Prove the following theorem: \\
let $f$ be closed and convex. Assume that it is differentiable on its domain. Then 
$\partial f(\xB) = \{ \nabla  f(\xB) \}$
for any $\xB \in \textrm{int}(\domf)$.
\end{excercise}

\begin{PROOF}{e2}
	It is obvious that $\partial f(\xB) \in \{ \nabla  f(\xB) \}$ for any $\xB \in \textrm{int}(\domf)$.

	Now we prove that there is no other vector in $\nabla f(\xB)$ except $\partial f(\xB)$.

	Assume that there is a vector $\bm{g} \in \partial f(\xB)$ and $\bm{g} \neq \nabla f(\xB)$.

	According to the definition of subdifferential, we have

	\[
	f(\bm{x}) \geq f(\xB_0) + \langle \bm{g}, \bm{x} - \xB_0 \rangle
	\]

	Let $\bm{x} = \xB_0 + at (\nabla f(\xB_0) - \bm{g})$, where $a \in \RBB$ and $t \in (0, 1)$.

	Therefore,

	\[
	f(\xB_0 + at(\xB - \xB_0)) = f(\xB_0) + at \langle \nabla f(\xB_0),  \nabla f(\xB_0) - \bm{g} \rangle + o(t) \geq f(\xB_0) + at \langle \nabla f(\xB_0),  \nabla f(\xB_0) - \bm{g} \rangle
	\]

	Which implies that

	\[
	\begin{aligned}
	&at \| \nabla f(\xB_0) - \bm{g} \|^2  + o(t) \geq 0 \\
	& \Leftrightarrow a \| \nabla f(\xB_0) - \bm{g} \|^2  + \frac{o(t)}{t} \geq 0 \\
	& \Rightarrow \lim_{t \to 0} a \| \nabla f(\xB_0) - \bm{g} \|^2  + \frac{o(t)}{t} \geq 0 \\
	& \Rightarrow a \| \nabla f(\xB_0) - \bm{g} \|^2  \geq 0 \\
	\end{aligned}
	\]

	Since $a \in \RBB$ and $a \neq 0$, we have

	\[
	\| \nabla f(\xB_0) - \bm{g} \|  = 0
	\]

	Which implies that $\bm{g} = \nabla f(\xB_0)$. 
	It is a contradiction.

	Therefore, $\partial f(\xB) = \{ \nabla f(\xB) \}$ for any $\xB \in \textrm{int}(\domf)$.
\end{PROOF}
\end{document}

