\documentclass{article}
\usepackage{hwopt}
\usepackage{amsmath}	% Package for AMS
\usepackage{amsthm}     % Package for AMS-therom
\usepackage{amssymb}	% Package for AMS-symbol
\usepackage{bm}

\newcommand{\xB}{\bm{x}}
\newcommand{\yB}{\bm{y}}
\newcommand{\RBB}{\mathbb{R}}
\newcommand{\FM}{\mathcal{F}}
\newcommand{\functiontype}[3]{\FM_{#1}^{#2,#3}(\RBB^n)}
\newcommand{\normgen}[1]{\left\| #1 \right\|}

%%%%%%%%%%%%%%%%%
%     Title     %
%%%%%%%%%%%%%%%%%
\title{Coursework (3) for \emph{Introductory Lectures on Optimization}}
\author{Zhou Nan \\ 3220102535}
\date{\today}

\begin{document}
\maketitle

\begin{excercise}\label{e0}
	Suppose that $f : \mathbb{R}^n \rightarrow \mathbb{R}$ is L-smooth ($C_L^{1,1}$), and  $\mu$-PL, that is 
	\[
	\textrm{$\mu$-PL:~~}\frac{1}{2} \| \nabla f(\xB) \|_2^2 \geq \mu \left( f(\xB) - f(\xB^*) \right),
	\]
	then GD iterates with step size $h_k = 1/L $ converge linearly, i.e.
	\[
	f(\xB_k) - f(\xB^*) \leq \left( 1 - \frac{\mu}{L} \right)^k \left(  f(\xB_0) - f(\xB^*)\right).
	\]
\end{excercise}

\begin{PROOF}{e0}
	According to the lemma 9, we have \\
	for any $\xB, \yB$ from $\RBB^n$,
	\[
	|f(\xB) - f(\yB) - \langle \nabla f(\xB), \xB - \yB \rangle | \leq \frac{L}{2} \| \xB - \yB \|_2^2.
	\]
	Since $\xB_{k+1} = \xB_k - \frac{1}{L} \nabla f(\xB_k)$, then 
	\[
	\begin{aligned}
	&|f(\xB_{k+1}) - f(\xB_k) - \langle \nabla f(\xB_k), \xB_{k+1} - \xB_k \rangle | 
	\leq \frac{L}{2} \| \xB_{k+1} - \xB_k \|_2^2.\\
	\Rightarrow &|f(\xB_{k+1}) - f(\xB_k) + \frac{1}{L} \| \nabla f(\xB_k) \|_2^2 | 
	\leq \frac{L}{2} \| \xB_{k+1} - \xB_k \|_2^2.\\
	\Rightarrow &|f(\xB_{k+1}) - f(\xB_k) + \frac{1}{L} \| \nabla f(\xB_k) \|_2^2 |
	\leq \frac{L}{2} \left( \frac{1}{L} \right)^2 \| \nabla f(\xB_k) \|_2^2.\\
	\Rightarrow &-\frac{3}{2L} \| \nabla f(\xB_k) \|_2^2 \leq f(\xB_{k+1}) - f(\xB_k) \leq -\frac{1}{2L} \| \nabla f(\xB_k) \|_2^2.
	\end{aligned}
	\]
	Since the function $f$ is $\mu$-PL, then 
	\[
	\frac{1}{2} \| \nabla f(\xB_k) \|_2^2 \geq \mu \left( f(\xB_k) - f(\xB^*) \right).
	\]
	Therefore,
	\[
	\begin{aligned}
	&L(f(\xB_{k+1}) - f(\xB_k)) + \mu (f(\xB_k) - f(\xB^*)) \\
	&\leq -\frac{1}{2} \| \nabla f(\xB_k) \|_2^2 + \frac{1}{2} \| \nabla f(\xB_k) \|_2^2 = 0.
	\end{aligned}
	\]
	Then,
	\[
	\begin{aligned}
	&f(\xB_{k+1}) - f(\xB_k) \leq -\frac{\mu}{L} (f(\xB_k) - f(\xB^*)) \\
	&f(\xB_{k+1}) - f(\xB_k) + f(\xB_k) - f(\xB^*) \leq (1 - \frac{\mu}{L}) (f(\xB_k) - f(\xB^*)).\\
	&f(\xB_{k+1}) - f(\xB^*) \leq (1 - \frac{\mu}{L}) (f(\xB_k) - f(\xB^*)).
	\end{aligned}
	\]
	Therefore,
	\[
	\begin{aligned}
	&f(\xB_{k+1}) - f(\xB^*) \leq (1 - \frac{\mu}{L}) (f(\xB_k) - f(\xB^*)) \\
	&f(\xB_k) - f(\xB^*) \leq (1 - \frac{\mu}{L}) (f(\xB_{k-1}) - f(\xB^*)) \\
	\Rightarrow &f(\xB_{k+1}) - f(\xB^*) \leq (1 - \frac{\mu}{L})^{2} (f(\xB_{k-1}) - f(\xB^*)).\\
	\Rightarrow &f(\xB_{k}) - f(\xB^*) \leq (1 - \frac{\mu}{L})^k (f(\xB_0) - f(\xB^*)).
	\end{aligned}
	\]
	
	
	
	
\end{PROOF}

\end{document}