\documentclass{article}
\usepackage{hwopt}
\usepackage{amsmath}	% Package for AMS
\usepackage{amsthm}     % Package for AMS-therom
\usepackage{amssymb}	% Package for AMS-symbol
\usepackage{bm}

\newcommand{\aB}{\bm{a}}
\newcommand{\bB}{\bm{b}}
\newcommand{\xB}{\bm{x}}
\newcommand{\yB}{\bm{y}}
\newcommand{\vB}{\bm{v}}
\newcommand{\uB}{\bm{u}}
\newcommand{\gB}{\bm{g}}
\newcommand{\RBB}{\mathbb{R}}
\newcommand{\FM}{\mathcal{F}}
\newcommand{\SM}{\mathcal{S}}
\newcommand{\LM}{\mathcal{L}}
\newcommand{\domf}{\textrm{dom}\;f}
\newcommand{\functiontype}[3]{\FM_{#1}^{#2,#3}(\RBB^n)}
\newcommand{\normgen}[1]{\left\| #1 \right\|}
\newcommand{\normone}[1]{\left\| #1 \right\|_1}
\newcommand{\strongconvextype}[2]{\SM_{#1}^{#2}(\RBB^n)}
\newcommand{\argmin}{\mathop{\rm argmin}}

%%%%%%%%%%%%%%%%%
%     Title     %
%%%%%%%%%%%%%%%%%
\title{Coursework (5) for \emph{Introductory Lectures on Optimization}}
\author{Zhou Nan \\ 3220102535}
\date{\today}

\begin{document}
\maketitle

\begin{excercise}\label{e0}
Prove the following theorem: \\
Let $\normgen{\cdot}$ be a vector norm in $\RBB^n$,  then 
\[
\partial \normgen{\cdot} = \left\{ V(\xB) \triangleq \left\{  \vB \in \RBB^n \big| \innerproduct{\vB}{\xB} = \normgen{\xB}, \normgen{\vB}_* \leq 1  \right\} \right\},
\]
where $\normgen{\vB}_*$ is the dual norm of $\normgen{\cdot}$, defined as
\[
\normgen{\vB}_* \triangleq \sup_{ \normgen{\uB} \leq 1} \innerproduct{\vB}{\uB}.
\]	
\end{excercise}
\begin{PROOF}{e0}
\begin{enumerate}
	\item Prove that $\partial \normgen{\cdot} \subseteq \left\{ V(\xB) \triangleq \left\{  \vB \in \RBB^n \big| \innerproduct{\vB}{\xB} = \normgen{\xB}, \normgen{\vB}_* \leq 1  \right\} \right\}$
	
	Let $\vB \in \partial \normgen{\xB}$, then we have

	\[
	\| \yB \| \geq \| \xB \| + \langle \vB, \yB - \xB \rangle, \forall \yB \in \RBB^n
	\]

	If $\yB = 0$, then we have

	\[
	\begin{aligned}
	\| \xB \| \leq \langle \vB, \xB \rangle \\
	\end{aligned}
	\]

	If $\yB = 2\xB$, then we have

	\[
	\begin{aligned}
	& 2 \| \xB \| \geq \| \xB \| + \langle \vB, \xB \rangle  \\
	& \Rightarrow  \| \xB \| \geq \langle \vB, \xB \rangle 
	\end{aligned}
	\]

	Therefore, we have $ \| \xB \| = \langle \vB, \xB \rangle $.

	Since 
	\[
		\normgen{\vB}_* \triangleq \sup_{ \normgen{\uB} \leq 1} \innerproduct{\vB}{\uB}.
	\]

	Then we have $1 \geq \| \uB \| \geq \| \xB \| + \langle \vB, \uB - \xB \rangle$.
	Which implies that $ 1 \geq \langle \vB, \xB \rangle + \langle \vB, \uB\rangle - \langle \vB, \xB \rangle = \langle \vB, \uB\rangle$.

	Therefore, we have $\normgen{\vB}_* \leq 1$, which implies that $\vB \in V(\xB)$.

	\item Prove that $\left\{ V(\xB) \triangleq \left\{  \vB \in \RBB^n \big| \innerproduct{\vB}{\xB} = \normgen{\xB}, \normgen{\vB}_* \leq 1  \right\} \right\} \subseteq \partial \normgen{\cdot}$
	
	Let $\vB \in V(\xB)$, then we have

	\[
	\begin{aligned}
	& \| \yB \| \geq \| \xB \| + \langle \vB, \yB - \xB \rangle \\
	& \Leftrightarrow \| \yB \|  \geq  \langle \vB, \xB \rangle + \langle \vB, \yB - \xB \rangle \\
	& \Leftrightarrow \| \yB \|  \geq  \langle \vB, \yB \rangle \\
	\end{aligned}
	\]

	Since $\normgen{\vB}_* \leq 1$, we have

	\[
	\begin{aligned}
	& \langle \vB, \yB \rangle \leq \normgen{\vB}_* \normgen{\yB} \leq \normgen{\yB} \\
	\end{aligned}
	\]

	Therefore, we have $\vB \in \partial \normgen{\xB}$, which implies that $\left\{ V(\xB) \triangleq \left\{  \vB \in \RBB^n \big| \innerproduct{\vB}{\xB} = \normgen{\xB}, \normgen{\vB}_* \leq 1  \right\} \right\} \subseteq \partial \normgen{\cdot}$.
	\item Therefore, we have $\partial \normgen{\cdot} = \left\{ V(\xB) \triangleq \left\{  \vB \in \RBB^n \big| \innerproduct{\vB}{\xB} = \normgen{\xB}, \normgen{\vB}_* \leq 1  \right\} \right\}$.
\end{enumerate}
\end{PROOF}
\newpage
\begin{excercise}\label{e1}
Write down the subdifferentials of following functions. \\
\begin{enumerate}
	\item $f(\xB) = |\xB|, \xB \in \RBB^1$.\vspace{8pt}
	\item $f(\xB) = \sum_{i=1}^{m} | \innerproduct{\aB_i}{\xB} - \bB_i|$.\vspace{8pt}
	\item $f(\xB) = \max_{1 \leq i \leq n} \xB^{(i)}$.\vspace{8pt}
	\item $f(\xB) = \normgen{\xB}$.\vspace{8pt}
	\item $f(\xB) = \normone{\xB} = \sum_{i=1}^{n} |\xB^{(i)}|$.
\end{enumerate}
\end{excercise}
\begin{SOLUTION}{e1}
\begin{enumerate}
	\item $f(\xB) = |\xB|, \xB \in \RBB^1$.
	\[
	\partial f(\xB) = \begin{cases}
		\{1\} & \xB > 0 \\
		\{-1\} & \xB < 0 \\
		[-1, 1] & \xB = 0
	\end{cases}
	\]
	\item $f(\xB) = \sum_{i=1}^{m} | \innerproduct{\aB_i}{\xB} - \bB_i|$.
	
	\[
	\partial f(\bm{x}) = \left\{ \sum_{i=1}^{m} s_{i} \aB_{i} \, \mid s_{i} \in 
	\begin{cases} 
	\{-1\}, & \langle \aB_i, \bm{x} \rangle < \bB_{i}, \\ 
	[-1, 1], & \langle \aB_i, \bm{x} \rangle = \bB_{i}, \\ 
	\{1\}, & \langle \aB_i, \bm{x} \rangle > \bB_{i}.
	\end{cases} 
	\right\}
	\]
	\item $f(\xB) = \max_{1 \leq i \leq n} \xB^{(i)}$.
	\[
		\partial f(\bm{x}) = \text{conv} \{ \bm{e}_{i} \mid \bm{x}^{(i)} = f(\bm{x}) \}
	\]
	\item $f(\xB) = \normgen{\xB}$.
	\[
	\partial f(\xB) = \left\{ \vB \mid \langle \vB, \xB \rangle = \normgen{\xB}, \normgen{\vB}_* \leq 1 \right\}
	\]
	\[
	\normgen{\vB}_* = \sup_{ \normgen{\uB} \leq 1} \innerproduct{\vB}{\uB}
	\]
	\item $f(\xB) = \normone{\xB} = \sum_{i=1}^{n} |\xB^{(i)}|$.
	\[
	\partial f(\xB) = \left\{ \sum_{i=1}^{n} \bm{s_{i}} \bm{e}_{i}  \mid \bm{s_{i}} \in 
	\begin{cases} 
	\{-1\}, & \quad \xB^{(i)} < 0, \\ 
	[-1, 1], & \quad \xB^{(i)} = 0, \\ 
	\{1\}, & \quad \xB^{(i)} > 0.
	\end{cases}\right\}
	\]
\end{enumerate}
\end{SOLUTION}
\newpage
\begin{excercise}\label{e2}
Please write down three sequences and prove that they satisfy the following conditions:
\[
 h_k > 0, h_k \to 0, \sum_{k=0}^{\infty} h_k = \infty.
 \]
\end{excercise}

\begin{SOLUTION}{e2}
\begin{enumerate}
	\item $h_k = \frac{1}{k}$
	\begin{itemize}
		\item $h_k > 0$: ✓ For all $k \geq 1$, $\frac{1}{k}$ is positive
		\item $h_k \to 0$: As $k \to \infty$, $\frac{1}{k} \to 0$ ✓
		\item $\sum_{k=0}^{\infty} h_k = \sum_{k=1}^{\infty} \frac{1}{k}$ is the harmonic series, which diverges to $\infty$ ✓
	\end{itemize}
	\item $h_k = \frac{1}{k^{\frac{1}{2}}}$
	\begin{itemize}
		\item $h_k > 0$: ✓ For all $k \geq 1$, $\frac{1}{k^{\frac{1}{2}}}$ is positive
		\item $h_k \to 0$: As $k \to \infty$, $\frac{1}{k^{\frac{1}{2}}} \to 0$ ✓
		\item $\sum_{k=1}^{\infty} \frac{1}{k^{\frac{1}{2}}}$ is a p-series with $p = \frac{1}{2}$, which diverges to $\infty$ ✓
	\end{itemize}
	\item $h_k = \frac{1}{k^{\frac{1}{3}}}$
	\begin{itemize}
		\item $h_k > 0$: ✓ For all $k \geq 1$, $\frac{1}{k^{\frac{1}{3}}}$ is positive
		\item $h_k \to 0$: As $k \to \infty$, $\frac{1}{k^{\frac{1}{3}}} \to 0$ ✓
		\item $\sum_{k=1}^{\infty} \frac{1}{k^{\frac{1}{3}}}$ is a p-series with $p = \frac{1}{3}$, which diverges to $\infty$ ✓
	\end{itemize}
\end{enumerate}
Proof why $\sum_{k=1}^{\infty} \frac{1}{k^p}$ diverges to $\infty$ when $p \leq 1$:

Since
\[
\int_1^{\infty} \frac{1}{x} dx = ln(x) |_1^{\infty} = \infty
\]
Then we have $\sum_{k=0}^{\infty} h_k = \sum_{k=1}^{\infty} \frac{1}{k}$ diverges to $\infty$.

Since 
\[
\frac{1}{k^p} \geq \frac{1}{k} \quad \text{for all } p \leq 1
\]

Then we have $\sum_{k=0}^{\infty} h_k = \sum_{k=1}^{\infty} \frac{1}{k^p}$ diverges to $\infty$ for all $p \leq 1$.

\end{SOLUTION}
\end{document}

